Start introducing notations for typing judgments.

F_mu/typing.v
@@ -1,53 +1,48 @@
 From iris_logrel.F_mu Require Export lang.
 
 Inductive type :=
-| TUnit : type
-| TProd : type → type → type
-| TSum : type → type → type
-| TArrow : type → type → type
-| TRec (τ : {bind 1 of type})
-| TVar (x : var)
-| TForall (τ : {bind 1 of type}).
+  | TUnit : type
+  | TProd : type → type → type
+  | TSum : type → type → type
+  | TArrow : type → type → type
+  | TRec (τ : {bind 1 of type})
+  | TVar (x : var)
+  | TForall (τ : {bind 1 of type}).
 
 Instance Ids_type : Ids type. derive. Defined.
 Instance Rename_type : Rename type. derive. Defined.
 Instance Subst_type : Subst type. derive. Defined.
 Instance SubstLemmas_typer : SubstLemmas type. derive. Qed.
 
+Reserved Notation "Γ ⊢ₜ e : τ" (at level 74, e, τ at next level).
+
 Inductive typed (Γ : list type) : expr → type → Prop :=
-| Var_typed x τ : Γ !! x = Some τ → typed Γ (Var x) τ
-| Unit_typed : typed Γ Unit TUnit
-| Pair_typed e1 e2 τ1 τ2 :
-    typed Γ e1 τ1 → typed Γ e2 τ2 → typed Γ (Pair e1 e2) (TProd τ1 τ2)
-| Fst_typed e τ1 τ2 : typed Γ e (TProd τ1 τ2) → typed Γ (Fst e) τ1
-| Snd_typed e τ1 τ2 : typed Γ e (TProd τ1 τ2) → typed Γ (Snd e) τ2
-| InjL_typed e τ1 τ2 : typed Γ e τ1 → typed Γ (InjL e) (TSum τ1 τ2)
-| InjR_typed e τ1 τ2 : typed Γ e τ2 → typed Γ (InjR e) (TSum τ1 τ2)
-| Case_typed e0 e1 e2 τ1 τ2 ρ :
-    typed Γ e0 (TSum τ1 τ2) →
-    typed (τ1 :: Γ) e1 ρ → typed (τ2 :: Γ) e2 ρ →
-    typed Γ (Case e0 e1 e2) ρ
-| Lam_typed e τ1 τ2 :
-    typed (τ1 :: Γ) e τ2 → typed Γ (Lam e) (TArrow τ1 τ2)
-| App_typed e1 e2 τ1 τ2 :
-    typed Γ e1 (TArrow τ1 τ2) → typed Γ e2 τ1 → typed Γ (App e1 e2) τ2
-| TLam_typed e τ :
-    typed (map (λ t, t.[ren (+1)]) Γ) e τ →
-    typed Γ (TLam e) (TForall τ)
-| TApp_typed e τ τ':
-    typed Γ e (TForall τ) → typed Γ (TApp e) (τ.[τ'/])
-| TFold e τ :
-    typed (map (λ t, t.[ren (+1)]) Γ) e τ →
-    typed Γ (Fold e) (TRec τ)
-| TUnfold e τ : typed Γ e (TRec τ) → typed Γ (Unfold e) (τ.[(TRec τ)/])
-.
+  | Var_typed x τ : Γ !! x = Some τ → Γ ⊢ₜ Var x : τ
+  | Unit_typed : Γ ⊢ₜ Unit : TUnit
+  | Pair_typed e1 e2 τ1 τ2 :
+     Γ ⊢ₜ e1 : τ1 → Γ ⊢ₜ e2 : τ2 → Γ ⊢ₜ Pair e1 e2 : TProd τ1 τ2
+  | Fst_typed e τ1 τ2 : Γ ⊢ₜ e : TProd τ1 τ2 → Γ ⊢ₜ Fst e : τ1
+  | Snd_typed e τ1 τ2 : Γ ⊢ₜ e : TProd τ1 τ2 → Γ ⊢ₜ Snd e : τ2
+  | InjL_typed e τ1 τ2 : Γ ⊢ₜ e : τ1 → Γ ⊢ₜ InjL e : TSum τ1 τ2
+  | InjR_typed e τ1 τ2 : Γ ⊢ₜ e : τ2 → Γ ⊢ₜ InjR e : TSum τ1 τ2
+  | Case_typed e0 e1 e2 τ1 τ2 ρ :
+     Γ ⊢ₜ e0 : TSum τ1 τ2 → τ1 :: Γ ⊢ₜ e1 : ρ → τ2 :: Γ ⊢ₜ e2 : ρ →
+     Γ ⊢ₜ Case e0 e1 e2 : ρ
+  | Lam_typed e τ1 τ2 : τ1 :: Γ ⊢ₜ e : τ2 → Γ ⊢ₜ Lam e : TArrow τ1 τ2
+  | App_typed e1 e2 τ1 τ2 : Γ ⊢ₜ e1 : TArrow τ1 τ2 → Γ ⊢ₜ e2 : τ1 → Γ ⊢ₜ App e1 e2 : τ2
+  | TLam_typed e τ : map (λ t, t.[ren (+1)]) Γ ⊢ₜ e : τ → Γ ⊢ₜ TLam e : TForall τ
+  | TApp_typed e τ τ' : Γ ⊢ₜ e : TForall τ → Γ ⊢ₜ TApp e : τ.[τ'/]
+  | TFold e τ : map (λ t, t.[ren (+1)]) Γ ⊢ₜ e : τ → Γ ⊢ₜ Fold e : TRec τ
+  | TUnfold e τ : Γ ⊢ₜ e : TRec τ → Γ ⊢ₜ Unfold e : τ.[TRec τ/]
+where "Γ ⊢ₜ e : τ" := (typed Γ e τ).
 
 Local Hint Extern 1 =>
-match goal with [H : context [length (map _ _)] |- _] => rewrite map_length in H end
-: typed_subst_invariant.
+  match goal with
+  | H : context [length (map _ _)] |- _ => rewrite map_length in H
+  end : typed_subst_invariant.
 
 Lemma typed_subst_invariant Γ e τ s1 s2 :
-  typed Γ e τ → (∀ x, x < length Γ → s1 x = s2 x) → e.[s1] = e.[s2].
+  Γ ⊢ₜ e : τ → (∀ x, x < length Γ → s1 x = s2 x) → e.[s1] = e.[s2].
 Proof.
   intros Htyped; revert s1 s2.
   assert (∀ {A} `{Ids A} `{Rename A}
@@ -60,21 +55,21 @@ Definition env_subst (vs : list val) (x : var) : expr :=
   from_option id (Var x) (of_val <$> vs !! x).
 
 Lemma typed_subst_head_simpl Δ τ e w ws :
-  typed Δ e τ -> length Δ = S (length ws) →
+  Δ ⊢ₜ e : τ → length Δ = S (length ws) →
   e.[# w .: env_subst ws] = e.[env_subst (w :: ws)].
 Proof.
   intros H1 H2.
   rewrite /env_subst. eapply typed_subst_invariant; eauto=> /= -[|x] ? //=.
   destruct (lookup_lt_is_Some_2 ws x) as [v' Hv]; first omega; simpl.
-    by rewrite Hv.
+  by rewrite Hv.
 Qed.
 
 Local Opaque eq_nat_dec.
 
 Lemma iter_up_subst_type (m : nat) (τ : type) (x : var) :
-    (iter m up (τ .: ids) x) =
+  iter m up (τ .: ids) x =
     if lt_dec x m then ids x else
-      if eq_nat_dec x m then τ.[ren (+m)] else ids (x - 1).
+    if eq_nat_dec x m then τ.[ren (+m)] else ids (x - 1).
 Proof.
   revert x τ.
   induction m; intros x τ; cbn.
