F_mu_ref_par/typing.v
@@ -1,17 +1,16 @@
 From iris_logrel.F_mu_ref_par Require Export lang.
 
 Inductive type :=
-| TUnit : type
-| TNat : type
-| TBool : type
-| TProd : type → type → type
-| TSum : type → type → type
-| TArrow : type → type → type
-| TRec (τ : {bind 1 of type})
-| TVar (x : var)
-| TForall (τ : {bind 1 of type})
-| Tref (τ : type)
-.
+  | TUnit : type
+  | TNat : type
+  | TBool : type
+  | TProd : type → type → type
+  | TSum : type → type → type
+  | TArrow : type → type → type
+  | TRec (τ : {bind 1 of type})
+  | TVar (x : var)
+  | TForall (τ : {bind 1 of type})
+  | Tref (τ : type).
 
 Instance Ids_type : Ids type. derive. Defined.
 Instance Rename_type : Rename type. derive. Defined.
@@ -25,64 +24,56 @@ Fixpoint binop_res_type (op : binop) : type :=
   end.
 
 Inductive EqType : type → Prop :=
-| EqTUnit : EqType TUnit
-| EqTNat : EqType TNat
-| EqTBool : EqType TBool
-| EqTProd τ τ' : EqType τ → EqType τ' → EqType (TProd τ τ')
-| EqSum τ τ' : EqType τ → EqType τ' → EqType (TSum τ τ')
-.
+  | EqTUnit : EqType TUnit
+  | EqTNat : EqType TNat
+  | EqTBool : EqType TBool
+  | EqTProd τ τ' : EqType τ → EqType τ' → EqType (TProd τ τ')
+  | EqSum τ τ' : EqType τ → EqType τ' → EqType (TSum τ τ').
+
+Reserved Notation "Γ ⊢ₜ e : τ" (at level 74, e, τ at next level).
 
 Inductive typed (Γ : list type) : expr → type → Prop :=
-| Var_typed x τ : Γ !! x = Some τ → typed Γ (Var x) τ
-| Unit_typed : typed Γ Unit TUnit
-| Nat_typed n : typed Γ (♯ n) TNat
-| Bool_typed b : typed Γ (♭ b) TBool
-| BinOp_typed op e1 e2 :
-    typed Γ e1 TNat → typed Γ e2 TNat →
-    typed Γ (BinOp op e1 e2) (binop_res_type op)
-| Pair_typed e1 e2 τ1 τ2 :
-    typed Γ e1 τ1 → typed Γ e2 τ2 → typed Γ (Pair e1 e2) (TProd τ1 τ2)
-| Fst_typed e τ1 τ2 : typed Γ e (TProd τ1 τ2) → typed Γ (Fst e) τ1
-| Snd_typed e τ1 τ2 : typed Γ e (TProd τ1 τ2) → typed Γ (Snd e) τ2
-| InjL_typed e τ1 τ2 : typed Γ e τ1 → typed Γ (InjL e) (TSum τ1 τ2)
-| InjR_typed e τ1 τ2 : typed Γ e τ2 → typed Γ (InjR e) (TSum τ1 τ2)
-| Case_typed e0 e1 e2 τ1 τ2 τ3 :
-    typed Γ e0 (TSum τ1 τ2) →
-    typed (τ1 :: Γ) e1 τ3 → typed (τ2 :: Γ) e2 τ3 →
-    typed Γ (Case e0 e1 e2) τ3
-| If_typed e0 e1 e2 τ :
-    typed Γ e0 TBool → typed Γ e1 τ → typed Γ e2 τ →
-    typed Γ (If e0 e1 e2) τ
-| Lam_typed e τ1 τ2 :
-    typed (TArrow τ1 τ2 :: τ1 :: Γ) e τ2 → typed Γ (Lam e) (TArrow τ1 τ2)
-| App_typed e1 e2 τ1 τ2 :
-    typed Γ e1 (TArrow τ1 τ2) → typed Γ e2 τ1 → typed Γ (App e1 e2) τ2
-| TLam_typed e τ :
-    typed (map (λ t, t.[ren (+1)]) Γ) e τ →
-    typed Γ (TLam e) (TForall τ)
-| TApp_typed e τ τ':
-    typed Γ e (TForall τ) → typed Γ (TApp e) (τ.[τ'/])
-| TFold e τ :
-    typed Γ e (τ.[(TRec τ)/]) →
-    typed Γ (Fold e) (TRec τ)
-| TUnfold e τ : typed Γ e (TRec τ) → typed Γ (Unfold e) (τ.[(TRec τ)/])
-| TFork e : typed Γ e TUnit → typed Γ (Fork e) TUnit
-| TAlloc e τ : typed Γ e τ → typed Γ (Alloc e) (Tref τ)
-| TLoad e τ : typed Γ e (Tref τ) → typed Γ (Load e) τ
-| TStore e e' τ :
-    typed Γ e (Tref τ) → typed Γ e' τ → typed Γ (Store e e') TUnit
-| TCAS e1 e2 e3 τ :
-    EqType τ →
-    typed Γ e1 (Tref τ) → typed Γ e2 τ → typed Γ e3 τ →
-    typed Γ (CAS e1 e2 e3) TBool
-.
+  | Var_typed x τ : Γ !! x = Some τ → Γ ⊢ₜ Var x : τ
+  | Unit_typed : Γ ⊢ₜ Unit : TUnit
+  | Nat_typed n : Γ ⊢ₜ ♯ n : TNat
+  | Bool_typed b : Γ ⊢ₜ ♭ b : TBool
+  | BinOp_typed op e1 e2 :
+     Γ ⊢ₜ e1 : TNat → Γ ⊢ₜ e2 : TNat → Γ ⊢ₜ BinOp op e1 e2 : binop_res_type op
+  | Pair_typed e1 e2 τ1 τ2 : Γ ⊢ₜ e1 : τ1 → Γ ⊢ₜ e2 : τ2 → Γ ⊢ₜ Pair e1 e2 : TProd τ1 τ2
+  | Fst_typed e τ1 τ2 : Γ ⊢ₜ e : TProd τ1 τ2 → Γ ⊢ₜ Fst e : τ1
+  | Snd_typed e τ1 τ2 : Γ ⊢ₜ e : TProd τ1 τ2 → Γ ⊢ₜ Snd e : τ2
+  | InjL_typed e τ1 τ2 : Γ ⊢ₜ e : τ1 → Γ ⊢ₜ InjL e : TSum τ1 τ2
+  | InjR_typed e τ1 τ2 : Γ ⊢ₜ e : τ2 → Γ ⊢ₜ InjR e : TSum τ1 τ2
+  | Case_typed e0 e1 e2 τ1 τ2 τ3 :
+     Γ ⊢ₜ e0 : TSum τ1 τ2 → τ1 :: Γ ⊢ₜ e1 : τ3 → τ2 :: Γ ⊢ₜ e2 : τ3 →
+     Γ ⊢ₜ Case e0 e1 e2 : τ3
+  | If_typed e0 e1 e2 τ :
+     Γ ⊢ₜ e0 : TBool → Γ ⊢ₜ e1 : τ → Γ ⊢ₜ e2 : τ → Γ ⊢ₜ If e0 e1 e2 : τ
+  | Lam_typed e τ1 τ2 :
+     TArrow τ1 τ2 :: τ1 :: Γ ⊢ₜ e : τ2 → Γ ⊢ₜ Lam e : TArrow τ1 τ2
+  | App_typed e1 e2 τ1 τ2 :
+     Γ ⊢ₜ e1 : TArrow τ1 τ2 → Γ ⊢ₜ e2 : τ1 → Γ ⊢ₜ App e1 e2 : τ2
+  | TLam_typed e τ :
+     map (λ t, t.[ren (+1)]) Γ ⊢ₜ e : τ → Γ ⊢ₜ TLam e : TForall τ
+  | TApp_typed e τ τ' : Γ ⊢ₜ e : TForall τ → Γ ⊢ₜ TApp e : τ.[τ'/]
+  | TFold e τ : Γ ⊢ₜ e : τ.[TRec τ/] → Γ ⊢ₜ Fold e : TRec τ
+  | TUnfold e τ : Γ ⊢ₜ e : TRec τ → Γ ⊢ₜ Unfold e : τ.[TRec τ/]
+  | TFork e : Γ ⊢ₜ e : TUnit → Γ ⊢ₜ Fork e : TUnit
+  | TAlloc e τ : Γ ⊢ₜ e : τ → Γ ⊢ₜ Alloc e : Tref τ
+  | TLoad e τ : Γ ⊢ₜ e : Tref τ → Γ ⊢ₜ Load e : τ
+  | TStore e e' τ : Γ ⊢ₜ e : Tref τ → Γ ⊢ₜ e' : τ → Γ ⊢ₜ Store e e' : TUnit
+  | TCAS e1 e2 e3 τ :
+     EqType τ → Γ ⊢ₜ e1 : Tref τ → Γ ⊢ₜ e2 : τ → Γ ⊢ₜ e3 : τ →
+     Γ ⊢ₜ CAS e1 e2 e3 : TBool
+where "Γ ⊢ₜ e : τ" := (typed Γ e τ).
 
 Local Hint Extern 1 =>
-match goal with [H : context [length (map _ _)] |- _] =>
-                rewrite map_length in H end : typed_subst_invariant.
+  match goal with
+  | H : context [length (map _ _)] |- _ => rewrite map_length in H
+  end : typed_subst_invariant.
 
 Lemma typed_subst_invariant Γ e τ s1 s2 :
-  typed Γ e τ → (∀ x, x < length Γ → s1 x = s2 x) → e.[s1] = e.[s2].
+  Γ ⊢ₜ e : τ → (∀ x, x < length Γ → s1 x = s2 x) → e.[s1] = e.[s2].
 Proof.
   intros Htyped; revert s1 s2.
   assert (∀ {A} `{Ids A} `{Rename A}
@@ -97,8 +88,8 @@ Definition env_subst (vs : list val) (x : var) : expr :=
   from_option id (Var x) (of_val <$> vs !! x).
 
 Lemma context_gen_weakening ξ Γ' Γ e τ :
-  typed (Γ' ++ Γ) e τ →
-  typed (Γ' ++ ξ ++ Γ) e.[iter (length Γ') up (ren (+ (length ξ)))] τ.
+  Γ' ++ Γ ⊢ₜ e : τ →
+  Γ' ++ ξ ++ Γ ⊢ₜ e.[iter (length Γ') up (ren (+ (length ξ)))] : τ.
 Proof.
   intros H1.
   remember (Γ' ++ Γ) as Ξ. revert Γ' Γ ξ HeqΞ.
@@ -127,11 +118,11 @@ Proof.
 Qed.
 
 Lemma context_weakening ξ Γ e τ :
-  typed Γ e τ → typed (ξ ++ Γ) e.[(ren (+ (length ξ)))] τ.
+  Γ ⊢ₜ e : τ → ξ ++ Γ ⊢ₜ e.[(ren (+ (length ξ)))] : τ.
 Proof. eapply (context_gen_weakening _ []). Qed.
 
 Lemma closed_context_weakening ξ Γ e τ :
-  (∀ f, e.[f] = e) → typed Γ e τ → typed (ξ ++ Γ) e τ.
+  (∀ f, e.[f] = e) → Γ ⊢ₜ e : τ → ξ ++ Γ ⊢ₜ e : τ.
 Proof. intros H1 H2. erewrite <- H1. by eapply context_weakening. Qed.
 
 Lemma n_closed_invariant n (e : expr) s1 s2 :
@@ -168,7 +159,7 @@ Proof.
 Qed.
 
 Lemma typed_n_closed Γ τ e :
-  typed Γ e τ -> (∀ f, e.[iter (length Γ) up f] = e).
+  Γ ⊢ₜ e : τ → (∀ f, e.[iter (length Γ) up f] = e).
 Proof.
   intros H. induction H => f; asimpl; unfold upn; simpl in *; auto with f_equal.
   - apply lookup_lt_Some in H. rewrite iter_up. destruct lt_dec; auto with omega.
@@ -183,17 +174,17 @@ Proof.
   intros H1 H2.
   rewrite /env_subst. eapply n_closed_invariant; eauto=> /= -[|x] ? //=.
   destruct (lookup_lt_is_Some_2 ws x) as [v' Hv]; first omega; simpl.
-    by rewrite Hv.
+  by rewrite Hv.
 Qed.
 
 Lemma typed_subst_head_simpl Δ τ e w ws :
-  typed Δ e τ -> length Δ = S (length ws) →
+  Δ ⊢ₜ e : τ → length Δ = S (length ws) →
   e.[# w .: env_subst ws] = e.[env_subst (w :: ws)].
 Proof.
   intros H1 H2.
   rewrite /env_subst. eapply typed_subst_invariant; eauto=> /= -[|x] ? //=.
   destruct (lookup_lt_is_Some_2 ws x) as [v' Hv]; first omega; simpl.
-    by rewrite Hv.
+  by rewrite Hv.
 Qed.
 
 Lemma n_closed_subst_head_simpl_2 n e w w' ws :
@@ -203,24 +194,24 @@ Proof.
   intros H1 H2.
   rewrite /env_subst. eapply n_closed_invariant; eauto => /= -[|[|x]] H3 //=.
   destruct (lookup_lt_is_Some_2 ws x) as [v' Hv]; first omega; simpl.
-    by rewrite Hv.
+  by rewrite Hv.
 Qed.
 
 Lemma typed_subst_head_simpl_2 Δ τ e w w' ws :
-  typed Δ e τ -> length Δ = 2 + (length ws) →
+  Δ ⊢ₜ e : τ → length Δ = 2 + length ws →
   e.[# w .: # w' .: env_subst ws] = e.[env_subst (w :: w' :: ws)].
 Proof.
   intros H1 H2.
   rewrite /env_subst. eapply typed_subst_invariant; eauto => /= -[|[|x]] H3 //=.
   destruct (lookup_lt_is_Some_2 ws x) as [v' Hv]; first omega; simpl.
-    by rewrite Hv.
+  by rewrite Hv.
 Qed.
 
 Local Opaque eq_nat_dec.
 
 Lemma iter_up_subst_type (m : nat) (τ : type) (x : var) :
-  (iter m up (τ .: ids) x) =
-  if lt_dec x m then ids x else
+  iter m up (τ .: ids) x =
+    if lt_dec x m then ids x else
     if eq_nat_dec x m then τ.[ren (+m)] else ids (x - 1).
 Proof.
   revert x τ.
@@ -236,7 +227,4 @@ Proof.
 Qed.
 
 Lemma empty_env_subst e : e.[env_subst []] = e.
-Proof.
-  replace (env_subst []) with (@ids expr _) by reflexivity.
-  asimpl; trivial.
-Qed.
+Proof. change (env_subst []) with (@ids expr _); by asimpl. Qed.
