stlc/typing.v
@@ -6,20 +6,21 @@ Inductive type :=
   | TSum : type → type → type
   | TArrow : type → type → type.
 
+Reserved Notation "Γ ⊢ₜ e : τ" (at level 74, e, τ at next level).
+
 Inductive typed (Γ : list type) : expr → type → Prop :=
-  | Var_typed x τ : Γ !! x = Some τ → typed Γ (Var x) τ
-  | Unit_typed : typed Γ Unit TUnit
+  | Var_typedx x τ : Γ !! x = Some τ → Γ ⊢ₜ Var x : τ
+  | Unit_typed : Γ ⊢ₜ Unit : TUnit
   | Pair_typed e1 e2 τ1 τ2 :
-     typed Γ e1 τ1 → typed Γ e2 τ2 → typed Γ (Pair e1 e2) (TProd τ1 τ2)
-  | Fst_typed e τ1 τ2 : typed Γ e (TProd τ1 τ2) → typed Γ (Fst e) τ1
-  | Snd_typed e τ1 τ2 : typed Γ e (TProd τ1 τ2) → typed Γ (Snd e) τ2
-  | InjL_typed e τ1 τ2 : typed Γ e τ1 → typed Γ (InjL e) (TSum τ1 τ2)
-  | InjR_typed e τ1 τ2 : typed Γ e τ2 → typed Γ (InjR e) (TSum τ1 τ2)
+     Γ ⊢ₜ e1 : τ1 → Γ ⊢ₜ e2 : τ2 → Γ ⊢ₜ Pair e1 e2 : TProd τ1 τ2
+  | Fst_typed e τ1 τ2 : Γ ⊢ₜ e : TProd τ1 τ2 → Γ ⊢ₜ Fst e : τ1
+  | Snd_typed e τ1 τ2 : Γ ⊢ₜ e : TProd τ1 τ2 → Γ ⊢ₜ Snd e : τ2
+  | InjL_typed e τ1 τ2 : Γ ⊢ₜ e : τ1 → Γ ⊢ₜ InjL e : TSum τ1 τ2
+  | InjR_typed e τ1 τ2 : Γ ⊢ₜ e : τ2 → Γ ⊢ₜ InjR e : TSum τ1 τ2
   | Case_typed e0 e1 e2 τ1 τ2 ρ :
-     typed Γ e0 (TSum τ1 τ2) →
-     typed (τ1 :: Γ) e1 ρ → typed (τ2 :: Γ) e2 ρ →
-     typed Γ (Case e0 e1 e2) ρ
-  | Lam_typed e τ1 τ2 :
-     typed (τ1 :: Γ) e τ2 → typed Γ (Lam e) (TArrow τ1 τ2)
+     Γ ⊢ₜ e0 : TSum τ1 τ2 → τ1 :: Γ ⊢ₜ e1 : ρ → τ2 :: Γ ⊢ₜ e2 : ρ →
+     Γ ⊢ₜ Case e0 e1 e2 : ρ
+  | Lam_typed e τ1 τ2 : τ1 :: Γ ⊢ₜ e : τ2 → Γ ⊢ₜ Lam e : TArrow τ1 τ2
   | App_typed e1 e2 τ1 τ2 :
-     typed Γ e1 (TArrow τ1 τ2) → typed Γ e2 τ1 → typed Γ (App e1 e2) τ2.
+     Γ ⊢ₜ e1 : TArrow τ1 τ2 → Γ ⊢ₜ e2 : τ1 → Γ ⊢ₜ App e1 e2 : τ2
+where "Γ ⊢ₜ e : τ" := (typed Γ e τ).
