F_mu_ref_par/soundness_unary.v
@@ -1,16 +1,16 @@
 From iris_logrel.F_mu_ref_par Require Export fundamental_unary.
 From iris.proofmode Require Import tactics pviewshifts.
-From iris.program_logic Require Import adequacy.
+From iris.program_logic Require Import ownership adequacy.
 
 Section Soundness.
-  Definition Σ := #[ auth.authGF heapUR ].
+  Let Σ := #[ auth.authGF heapUR ].
 
   Definition free_type_context: varC -n> valC -n> iPropG lang Σ := λne x y,
     True%I.
 
   Lemma wp_soundness e τ :
-    typed [] e τ →
-    ownership.ownP ∅ ⊢ WP e {{v, ∃ H : heapIG Σ,
+    [] ⊢ₜ e : τ →
+    ownP ∅ ⊢ WP e {{v, ∃ H : heapIG Σ,
       interp (nroot .@ "Fμ,ref,par" .@ 1) τ free_type_context v }}.
   Proof.
     iIntros {H1} "Hemp".
@@ -26,14 +26,14 @@ Section Soundness.
   Qed.
 
   Theorem Soundness e τ :
-    typed [] e τ →
+    [] ⊢ₜ e : τ →
     ∀ e' thp h, rtc step ([e], (of_heap ∅)) (e' :: thp, h) →
               ¬reducible e' h → is_Some (to_val e').
   Proof.
     intros H1 e' thp h Hstp Hnr.
     eapply wp_soundness in H1; eauto.
-    edestruct (@wp_adequacy_reducible lang (globalF Σ) ⊤ (λ v, (∃ H,
-        @interp Σ H (nroot .@ "Fμ,ref,par" .@ 1) τ free_type_context v)%I)
+    edestruct (@wp_adequacy_reducible lang (globalF Σ) ⊤ (λ v, ∃ H,
+        @interp Σ H (nroot .@ "Fμ,ref,par" .@ 1) τ free_type_context v)%I
       e e' (e' :: thp) ∅ ∅ h) as [Ha|Ha]; eauto; try tauto.
     - apply ucmra_unit_valid.
     - iIntros "[Hp Hg]". by iApply H1.
